mon.v
@@ -97,10 +97,6 @@ Section marking_definitions.
     by rewrite -already_marked_op.
   Qed.
 
-  Lemma new_marking_dom m x :
-    dom (gset loc) (m ⋅ {[x := ()]}) = dom (gset loc) m ∪ {[x]}.
-  Proof. by rewrite dom_op dom_singleton_L. Qed.
-
 End marking_definitions.
 
 (* The monoid representing graphs *)
@@ -134,40 +130,38 @@ Definition child_to_val (c : option loc) : val :=
 Definition children_to_val (ch : option loc * option loc) : val :=
   (child_to_val (ch.1), child_to_val (ch.2)).
 
+Lemma children_to_val_is_val (c c' : option loc) :
+  to_val (child_to_val c, child_to_val c') =
+  Some (child_to_val c, child_to_val c')%V.
+Proof. by destruct c; destruct c'. Qed.
+
+Definition marked_graph := gmap loc (bool * (option loc * option loc)).
+Identity Coercion marked_graph_gmap: marked_graph >-> gmap.
+
 Definition of_graph_elem (G : Gmon) i v
-  : option (option loc * option loc) :=
+  : option (bool * (option loc * option loc)) :=
   match Gmon_graph G !! i with
-  | Some w => Some w
-  | None => Some v
+  | Some w => Some (true, w)
+  | None => Some (false,v)
   end.
 
-Definition of_graph (g : graph loc) (G : Gmon) : graph loc :=
+Definition of_graph (g : graph loc) (G : Gmon) : marked_graph :=
   map_imap (of_graph_elem G) g.
-
-Definition is_marked_in (G : Gmon) x : bool :=
-  if mapset_elem_of_dec x (dom (gset _) G) then true else false.
 
 (* facts *)
 
 Global Instance Gmon_graph_proper : Proper ((≡) ==> (=)) Gmon_graph.
 Proof. solve_proper. Qed.
 
-Definition is_marked_in_op G x w : is_marked_in (G ⋅ {[x := w]}) x = true.
-Proof.
-  unfold is_marked_in. destruct mapset_elem_of_dec as [Hd|Hd]; trivial.
-  exfalso; apply Hd.
-  rewrite dom_op elem_of_union dom_singleton elem_of_singleton; auto.
-Qed.
-
 Lemma new_Gmon_dom (G : Gmon) x w :
   dom (gset loc) (G ⋅ {[x := w]}) = dom (gset loc) G ∪ {[x]}.
 Proof. by rewrite dom_op dom_singleton_L. Qed.
 
-Definition of_graph_empty (g : graph loc) : of_graph g ∅ = g.
+Definition of_graph_empty (g : graph loc) :
+  of_graph g ∅ = fmap (λ x, (false, x)) g.
 Proof.
   apply: map_eq => i.
-  rewrite lookup_imap /of_graph_elem lookup_omap lookup_empty //=.
-  case _ : (g !! i) => //=.
+  rewrite lookup_imap /of_graph_elem lookup_fmap lookup_omap //.
 Qed.
 
 Section definitions.
@@ -179,15 +173,15 @@ Section definitions.
   Global Instance own_graph_proper q : Proper ((≡) ==> (⊣⊢)) (own_graph q).
   Proof. solve_proper. Qed.
 
+  Definition heap_owns (M : marked_graph) (markings : gmap loc loc) : iProp Σ :=
+    ([★ map] l ↦ v ∈ M, ∃ (m : loc), markings !! l = Some m
+       ★ l ↦ (#m, children_to_val (v.2)) ★ m ↦ #(v.1))%I.
+
   Definition graph_inv (g : graph loc) (markings : gmap loc loc) : iProp Σ :=
     (∃ (G : Gmon) (M : markingUR),
-       own graph_name (● Some (1%Qp, G))
-       ★ own graph_marking_name (● M)
-          ★ ([★ map] l ↦ v ∈ (of_graph g G),
-               ∃ (m : loc), markings !! l = Some m
-                 ★ l ↦ (#m, children_to_val v) ★ m ↦ #(is_marked_in G l))
-          ★ ■ (dom (gset _) M = dom (gset _) G)
-          ★ ■ (strict_subgraph g (Gmon_graph G))
+       own graph_name (● Some (1%Qp, G)) ★ own graph_marking_name (● M)
+       ★ heap_owns (of_graph g G) markings
+       ★ dom (gset _) M = dom (gset _) G ★ ■ (strict_subgraph g (Gmon_graph G))
     )%I.
 
   Global Instance graph_inv_timeless g Mrk : TimelessP (graph_inv g Mrk).
@@ -210,13 +204,10 @@ Section graph_ctx_alloc.
 
   Lemma graph_ctx_alloc (E : coPset) (g : graph loc) (markings : gmap loc loc)
         (HNE : (nclose graphN) ⊆ E)
-    :
-      ([★ map] l ↦ v ∈ g,
-       ∃ (m : loc), markings !! l = Some m ★ l ↦ (#m, children_to_val v)
-                                    ★ m ↦ #false)
-      ={E}=>
-      ∃ (Ig : graphG Σ) (κ : gname),
-        cinv_own κ 1 ★ graph_ctx κ g markings ★ own_graph 1%Qp ∅.
+  : ([★ map] l ↦ v ∈ g, ∃ (m : loc), markings !! l = Some m
+       ★ l ↦ (#m, children_to_val v) ★ m ↦ #false)
+     ={E}=> ∃ (Ig : graphG Σ) (κ : gname), cinv_own κ 1 ★ graph_ctx κ g markings
+             ★ own_graph 1%Qp ∅.
   Proof.
     iIntros "H1".
     iVs (own_alloc (● (∅ : markingUR))) as (mn) "H2"; first done.
@@ -230,7 +221,7 @@ Section graph_ctx_alloc.
     { unfold graph_inv. iExists ∅, ∅.
       iFrame "H2 H31".
       iSplitL; [|iSplit; iPureIntro].
-      - rewrite of_graph_empty {2}big_sepM_proper; eauto.
+      - rewrite /heap_owns of_graph_empty  big_sepM_fmap; eauto.
       - by rewrite ?dom_empty_L.
       - rewrite /Gmon_graph omap_empty; apply strict_subgraph_empty. }
     iVs (cinv_alloc _ graphN with "[H]") as (κ) "[Hinv key]".
@@ -260,37 +251,59 @@ Lemma mark_update_lookup_ne_base (G : Gmon) x i v :
   i ≠ x → ({[x := Excl v]} ⋅ G) !! i = G !! i.
 Proof. intros H. by rewrite lookup_op lookup_singleton_ne //= left_id_L. Qed.
 
-Lemma of_graph_dom g γ : ✓ γ → dom (gset _) (of_graph g γ) = dom (gset _) g.
+Lemma of_graph_dom g G : dom (gset _) (of_graph g G) = dom (gset _) g.
 Proof.
-  intros H1. apply mapset_eq=>i.
-  rewrite ?elem_of_dom lookup_imap. case _ : (g !! i) => [x|]; simpl; trivial.
-  split; eauto. rewrite /of_graph_elem /Gmon_graph lookup_omap.
-  case _ : (γ !! i) => [[]|] //=; eauto.
+  apply mapset_eq=>i.
+  rewrite ?elem_of_dom lookup_imap /of_graph_elem lookup_omap.
+  case _ : (g !! i) => [x|]; case _ : (G !! i) => [[]|] //=; split;
+  intros [? Hcn]; inversion Hcn; eauto.
 Qed.
 
-(** Conversion to heaps and back *)
+Lemma in_dom_of_graph (g : graph loc) (G : Gmon) x (b : bool) v :
+  ✓ G → of_graph g G !! x = Some (b, v) → b ↔ x ∈ dom (gset _) G.
+Proof.
+  rewrite /of_graph /of_graph_elem lookup_imap lookup_omap elem_of_dom.
+  intros Hvl; specialize (Hvl x); revert Hvl;
+  case _ : (g !! x) => [?|]; case _ : (G !! x) => [[] ?|] //=;
+    intros Hvl; inversion Hvl; try (inversion 1; subst); split;
+    try (inversion 1; fail); try (intros [? Hcn]; inversion Hcn; fail);
+    subst; eauto.
+Qed.
+
 Global Instance of_graph_proper g : Proper ((≡) ==> (=)) (of_graph g).
 Proof. solve_proper. Qed.
 
-Lemma mark_update_lookup g γ x v :
+
+Lemma mark_update_lookup (g : graph loc) (G : Gmon) x v :
   x ∈ dom (gset _) g →
-  ✓ ({[x := Excl v]} ⋅ γ) →
-  of_graph g ({[x := Excl v]} ⋅ γ) !! x = Some v.
+  ✓ ((x [↦] v) ⋅ G) → of_graph g ((x [↦] v) ⋅ G) !! x = Some (true, v).
 Proof.
   rewrite elem_of_dom /is_Some. intros [w H1] H2.
   rewrite /of_graph /of_graph_elem lookup_imap H1 lookup_omap; simpl.
   rewrite mark_update_lookup_base; trivial.
 Qed.
 
-Lemma mark_update_lookup_ne g γ x i v :
-  i ≠ x → of_graph g ({[x := Excl v]} ⋅ γ) !! i = (of_graph g γ) !! i.
+Lemma mark_update_lookup_ne (g : graph loc) (G : Gmon) x i v :
+  i ≠ x → of_graph g ((x [↦] v) ⋅ G) !! i = (of_graph g G) !! i.
 Proof.
   intros H. rewrite /of_graph /of_graph_elem ?lookup_imap ?lookup_omap; simpl.
   rewrite mark_update_lookup_ne_base //=.
 Qed.
 
 Section graph.
-  Context `{Ih : heapG Σ, Ig : graphG Σ}.
+  Context `{heapG Σ, graphG Σ}.
+
+  Lemma own_graph_valid q G : own_graph q G ⊢ ✓ G.
+  Proof.
+    iIntros "H". unfold own_graph.
+    by iDestruct (own_valid with "#H") as %[_ ?].
+  Qed.
+
+  Lemma auth_own_graph_valid q G : own graph_name (● Some (q, G))  ⊢ ✓ G.
+  Proof.
+    iIntros "H". unfold own_graph.
+    by iDestruct (own_valid with "#H") as %[_ [_ ?]].
+  Qed.
 
   Lemma whole_frac (G G' : Gmon):
     own graph_name (● Some (1%Qp, G)) ★ own_graph 1 G' ⊢ G = G'.
@@ -337,41 +350,32 @@ Section graph.
     iPureIntro.
   Admitted.
 
-  Lemma graph_open g markings (G : Gmon) x : x ∈ dom (gset _) g →
+  Lemma graph_open (g :graph loc) (markings : gmap loc loc) (G : Gmon) x
+  : x ∈ dom (gset _) g →
+    own graph_name (● Some (1%Qp, G)) ★ heap_owns (of_graph g G) markings ⊢
     own graph_name (● Some (1%Qp, G))
-    ★ ([★ map] l ↦ v ∈ (of_graph g G),
-         ∃ (m : loc), markings !! l = Some m ★ l ↦ (#m, children_to_val v)
-           ★ m ↦ #(is_marked_in G l))
-      ⊢ own graph_name (● Some (1%Qp, G))
-      ★ ([★ map] l ↦ v ∈ delete x (of_graph g G),
-         ∃ (m : loc), markings !! l = Some m ★ l ↦ (#m, children_to_val v)
-           ★ m ↦ #(is_marked_in G l))
-      ★ (∃ u, (of_graph g G !! x = Some u)
-           ★ ∃ (m : loc), markings !! x = Some m ★ x ↦ (#m, children_to_val u)
-               ★ m ↦ #(is_marked_in G x)).
+    ★ heap_owns (delete x (of_graph g G)) markings
+    ★ (∃ u : bool * (option loc * option loc), (of_graph g G !! x = Some u)
+         ★ ∃ (m : loc), markings !! x = Some m ★ x ↦ (#m, children_to_val (u.2))
+           ★ m ↦ #(u.1)).
   Proof.
-    iIntros (H1) "(Hg & Ha)".
-    iDestruct (@own_valid with "#Hg") as %[_ [_ Hv]].
+    iIntros (Hx) "(Hg & Ha)".
     assert (Hid : x ∈ dom (gset _) (of_graph g G)) by (by rewrite of_graph_dom).
     revert Hid; rewrite elem_of_dom /is_Some. intros [y Hy].
-    rewrite -{1}(insert_id _ _ _ Hy) -insert_delete.
+    rewrite /heap_owns -{1}(insert_id _ _ _ Hy) -insert_delete.
     rewrite big_sepM_insert; [|apply lookup_delete_None; auto].
     iDestruct "Ha" as "[H $]". iFrame "Hg". iExists _; eauto.
   Qed.
 
   Lemma graph_close g markings G x :
-    ([★ map] l ↦ v ∈ delete x (of_graph g G),
-         ∃ (m : loc), markings !! l = Some m ★ l ↦ (#m, children_to_val v)
-                                      ★ m ↦ #(is_marked_in G l))
-      ★ (∃ u, (of_graph g G !! x = Some u)
-           ★ ∃ (m : loc), markings !! x = Some m ★ x ↦ (#m, children_to_val u)
-                                               ★ m ↦ #(is_marked_in G x))
-      ⊢ ([★ map] l ↦ v ∈ (of_graph g G),
-         ∃ (m : loc), markings !! l = Some m ★ l ↦ (#m, children_to_val v)
-           ★ m ↦ #(is_marked_in G l)).
+    heap_owns (delete x (of_graph g G)) markings
+    ★ (∃ u : bool * (option loc * option loc), (of_graph g G !! x = Some u)
+        ★ ∃ (m : loc), markings !! x = Some m ★ x ↦ (#m, children_to_val (u.2))
+            ★ m ↦ #(u.1))
+    ⊢ heap_owns (of_graph g G) markings.
   Proof.
     iIntros "[Ha Hl]". iDestruct "Hl" as (u) "[Hu Hl]". iDestruct "Hu" as %Hu.
-    rewrite -{2}(insert_id _ _ _ Hu) -insert_delete.
+    rewrite /heap_owns -{2}(insert_id _ _ _ Hu) -insert_delete.
     rewrite big_sepM_insert; [|apply lookup_delete_None; auto]. by iFrame "Ha".
   Qed.
 
@@ -401,6 +405,16 @@ Section graph.
 End graph.
 
 (* Graph properties *)
+
+Lemma delete_marked g G x w :
+  delete x (of_graph g G) = delete x (of_graph g ((x [↦] w) ⋅ G)).
+Proof.
+  apply: map_eq => i. destruct (decide (i = x)).
+  - subst; by rewrite ?lookup_delete.
+  - rewrite ?lookup_delete_ne //= /of_graph /of_graph_elem ?lookup_imap
+      ?lookup_omap; case _ : (g !! i) => [v|] //=.
+    by rewrite lookup_op lookup_singleton_ne //= left_id_L.
+Qed.
 
 Lemma in_dom_conv (G G' : Gmon) x : ✓ (G ⋅ G') → x ∈ dom (gset _) (Gmon_graph G)
   → (Gmon_graph (G ⋅ G')) !! x = (Gmon_graph G) !! x.
@@ -669,4 +683,86 @@ Proof.
  - split; trivial. intros z v. in_dom_Gmon_graph. intros ? [Hl|Hl]; subst.
     + rewrite get_left_singleton in Hl; inversion Hl.
     + rewrite get_right_singleton in Hl; inversion Hl.
+Qed.
+
+Lemma update_valid (G : Gmon) x v w : ✓ ((x [↦] v) ⋅ G) → ✓ ((x [↦] w) ⋅ G).
+Proof.
+  intros Hvl i; specialize (Hvl i); revert Hvl.
+  rewrite ?lookup_op. destruct (decide (i = x)).
+  - subst; rewrite ?lookup_singleton; case _ : (G !! x); done.
+  - rewrite ?lookup_singleton_ne //=.
+Qed.
+
+Lemma of_graph_unmarked (g : graph loc) (G : Gmon) x v :
+  of_graph g G !! x = Some (false, v) → g !! x = Some v.
+Proof.
+  rewrite lookup_imap /of_graph_elem lookup_omap.
+  case _ : (g !! x); case _ : (G !! x) => [[]|]; by inversion 1.
+Qed.
+Lemma get_lr_disj (G G' : Gmon) i : ✓ (G ⋅ G') →
+  (get_left (Gmon_graph (G ⋅ G')) i = get_left (Gmon_graph G) i ∧
+   get_right (Gmon_graph (G ⋅ G')) i = get_right (Gmon_graph G) i ∧
+   get_left (Gmon_graph G') i = None ∧
+   get_right (Gmon_graph G') i = None) ∨
+  (get_left (Gmon_graph (G ⋅ G')) i = get_left (Gmon_graph G') i ∧
+   get_right (Gmon_graph (G ⋅ G')) i = get_right (Gmon_graph G') i ∧
+   get_left (Gmon_graph G) i = None ∧
+   get_right (Gmon_graph G) i = None).
+Proof.
+  intros Hvl. specialize (Hvl i). revert Hvl.
+  rewrite /get_left /get_right /Gmon_graph ?lookup_omap ?lookup_op.
+  case _ : (G !! i) => [[]|]; case _ : (G' !! i) => [[]|]; inversion 1;
+    simpl; auto.
+Qed.
+Lemma mark_update_strict_subgraph (g : graph loc) (G G' : Gmon) : ✓ (G ⋅ G') →
+  strict_subgraph g (Gmon_graph G) ∧ strict_subgraph g (Gmon_graph G') ↔
+  strict_subgraph g (Gmon_graph (G ⋅ G')).
+Proof.
+  intros Hvl; split.
+  - intros [HG HG'] i.
+  destruct (get_lr_disj G G' i) as [(-> & -> & _ & _)|(-> & -> & _ & _)]; eauto.
+  - intros HGG; split => i.
+    + destruct (get_lr_disj G G' i) as [(<- & <- & _ & _)|(_ & _ & -> & ->)];
+       eauto using strict_sub_children_None.
+    + destruct (get_lr_disj G G' i) as [(_ & _ & -> & ->)|(<- & <- & _ & _)];
+       eauto using strict_sub_children_None.
+Qed.
+Lemma strinct_subgraph_singleton (g : graph loc) x v :
+  x ∈ dom (gset _) g → (∀ w, g !! x = Some w → strict_sub_children w v)
+  ↔ strict_subgraph g (Gmon_graph (x [↦] v)).
+Proof.
+  rewrite elem_of_dom; intros [u Hu]; split.
+  - move => /(_ _ Hu) Hgw i.
+    rewrite /get_left /get_right /Gmon_graph lookup_omap.
+    destruct (decide (i = x)); subst.
+    + by rewrite Hu lookup_singleton; simpl.
+    + rewrite lookup_singleton_ne; auto. by case _ : (g !! i) => [[[?|] [?|]]|].
+  - intros Hg w Hw; specialize (Hg x). destruct v as [v1 v2]; simpl. revert Hg.
+    rewrite Hu in Hw; inversion Hw; subst.
+    by rewrite get_left_singleton get_right_singleton /get_left /get_right Hu.
+Qed.
+Lemma mark_strict_subgraph (g : graph loc) (G : Gmon) x v :
+  ✓ ((x [↦] v) ⋅ G) → x ∈ dom (gset positive) g →
+  of_graph g G !! x = Some (false, v) → strict_subgraph g (Gmon_graph G) →
+  strict_subgraph g (Gmon_graph ((x [↦] v) ⋅ G)).
+Proof.
+  intros Hvl Hdx Hx Hsg. apply mark_update_strict_subgraph; try split; eauto.
+  eapply strinct_subgraph_singleton; erewrite ?of_graph_unmarked; eauto.
+  inversion 1; auto using strict_sub_children_refl.
+Qed.
+Lemma update_strict_subgraph (g : graph loc) (G : Gmon) x v w :
+  ✓ ((x [↦] v) ⋅ G) → x ∈ dom (gset positive) g →
+  strict_subgraph g (Gmon_graph ((x [↦] w) ⋅ G)) →
+  strict_sub_children w v →
+  strict_subgraph g (Gmon_graph ((x [↦] v) ⋅ G)).
+Proof.
+  intros Hvl Hdx Hx Hsc1 Hsc2.
+  apply mark_update_strict_subgraph in Hx; eauto using update_valid.
+  destruct Hx as [Hx1 Hx2].
+  apply mark_update_strict_subgraph; try split; try tauto.
+  pose proof (proj1 (elem_of_dom _ _) Hdx) as [u Hu].
+  eapply strinct_subgraph_singleton in Hx1; eauto.
+  apply strinct_subgraph_singleton; trivial.
+  intros u' Hu'; rewrite Hu in Hu'; inversion Hu'; subst.
+  intuition eauto using strict_sub_children_trans.
 Qed.
